SystemF2Effect: sort out store well formedness relations
Ignore-this: 8261fd7f6d38bafe98b222d7546a3ce3

darcs-hash:20130213031609-08f32-e7c187cd236034df66a6427bbce98181bf5e5665

devel/Iron/SystemF2Effect/Store/Bind.v
@@ -1,6 +1,7 @@
 
 Require Export Iron.SystemF2Effect.Value.
 Require Import Iron.SystemF2Effect.Value.TyJudge.WeakStProps.
+Require Import Iron.SystemF2Effect.Value.TyJudge.TypeKind.
 
 
 (* Store bindings are the primitive objects we keep in the store.
@@ -55,5 +56,65 @@ Proof.
  intros. inverts H. eauto.
 Qed.
 Hint Resolve typeb_stprops_snoc.
+
+
+(******************************************************************************)
+(* Well typed store.
+   All bindings are well typed. *)
+Definition STORET (se: stenv) (sp: stprops) (ss: store)
+ := Forall2 (TYPEB nil nil se sp) ss se.
+Hint Unfold STORET.
+
+
+(* Weaken store properties in store typing judgement. *)
+Lemma storet_weak_stprops
+ :  forall se sp ss p
+ ,  STORET se sp ss
+ -> STORET se (sp :> SRegion p) ss.
+Proof.
+ intros.
+ unfold STORET in *.
+ eapply Forall2_impl.
+  intros. eapply typeb_stprops_cons. eauto.
+ auto.
+Qed.
+Hint Resolve storet_weak_stprops.
+
+
+(* Extended store is well typed under extended store environment *)
+Lemma storet_snoc
+ :  forall se sp ss r1 v1 t2
+ ,  TYPEV  nil nil se sp v1 t2
+ -> STORET                                     se  sp                   ss
+ -> STORET (tRef (TCap (TyCapRegion r1)) t2 <: se) sp (StValue r1 v1 <: ss).
+Proof.
+ intros.
+ set (tRef' := tRef (TCap (TyCapRegion r1)) t2).
+
+ assert (TYPEB nil nil (tRef' <: se) sp (StValue r1 v1) tRef').
+  apply TbValue.
+   apply typev_stenv_snoc.
+    subst tRef'.
+    assert (closedT t2).
+     unfold closedT.
+     rrwrite (0 = @length ki nil).
+     apply (kind_wfT nil sp t2 KData).
+
+     (* NOTE: This one has to be done manually to instantiate existentials *)
+     apply (typex_kind_type nil nil se sp (XVal v1) t2 (TBot KEffect)).
+    auto. auto. auto.
+     
+ assert (Forall2 (TYPEB nil nil (tRef' <: se) sp) ss se).
+  lets D: (@Forall2_impl stbind ty) 
+                (TYPEB nil nil se sp) 
+                (TYPEB nil nil (tRef' <: se) sp)
+                ss se H0.
+  intros.
+  apply typeb_stenv_snoc.
+   auto.
+   subst tRef'. eauto.
+  auto. auto.
+Qed.
+Hint Resolve storet_snoc.
 
 
