devel/Iron/SystemF2Effect/Store/Wf.v
@@ -1,0 +1,108 @@
+
+Require Export Iron.SystemF2Effect.Store.Bind.
+Require Export Iron.SystemF2Effect.Step.Frame.
+
+
+(******************************************************************************)
+(* Store typing models the store.
+   All types in the store typing have a corresponding binding in the store.
+   We don't want entries in the store typing that don't have corresponding
+   bindings in the store. *)
+
+Definition STOREM (se: stenv) (ss: store)
+ := length se = length ss.
+Hint Unfold STOREM.
+
+
+(* Extended store environment models the extended store *)
+Lemma storem_snoc
+ :  forall se ss t stv
+ ,  STOREM se ss
+ -> STOREM (t <: se) (stv <: ss).
+Proof.
+ intros.
+ unfold STOREM.
+ have (length se = length ss). 
+ burn.
+Qed.
+Hint Resolve storem_snoc.
+
+
+(*****************************************************************************)
+(* All region handles on frame stack are in store properties.
+
+   We don't require the other way, forcing all store properties to be in 
+   the frame stack. This is because we need to be able to pop a Use frame and
+   still have any region handles in the expression being well typed, along with
+   dangling references into that region. *)
+
+Definition STOREP  (sp : stprops) (fs : stack)
+ := forall n, In (FUse n) fs -> In (SRegion n) sp.
+
+
+(* Weaken frame stack in store properties. *)
+Lemma storep_cons
+ :  forall sp fs p
+ ,  STOREP sp fs
+ -> STOREP (sp :> SRegion p) (fs :> FUse p).
+Proof.
+ unfold STOREP in *.
+ - intros.
+   have HN: (n = p \/ ~(n = p)).
+   inverts HN.
+   + simpl. auto.
+   + assert (In (FUse n) fs).
+      eapply in_tail.
+      have (FUse n <> FUse p) by congruence.
+      eauto. auto.
+     eapply in_split.
+      left. eapply H. auto.
+Qed.
+Hint Resolve storep_cons.
+
+
+(******************************************************************************)
+(* Well formed store. *)
+Definition WfS  (se: stenv) (sp: stprops)  (ss: store)
+ := Forall closedT se
+ /\ STOREM se    ss
+ /\ STORET se sp ss.
+Hint Unfold WfS.
+
+
+(* Well formed store and frame stack. *)
+Definition WfFS (se : stenv) (sp : stprops) (ss : store) (fs : stack) 
+ := Forall closedT se
+ /\ STOREM se ss
+ /\ STORET se sp ss
+ /\ STOREP sp fs.
+
+
+Lemma wfFS_wfS 
+ :  forall se sp ss fs
+ ,  WfFS   se sp ss fs
+ -> WfS    se sp ss.
+Proof. firstorder. Qed.
+
+
+Lemma wfFS_fuse_sregion
+ :  forall se sp ss fs p
+ ,  WfFS se sp ss fs
+ -> In (FUse p)    fs
+ -> In (SRegion p) sp.
+Proof. firstorder. Qed.
+
+
+(* Weaken frame stack in WfFS *)
+Lemma wffs_sregion_cons
+ :  forall se sp ss fs p
+ ,  WfFS se sp ss fs
+ -> WfFS se (sp :> SRegion p) ss (fs :> FUse p).
+Proof. 
+ intros.
+ unfold WfFS. 
+ inverts H. inverts H1. inverts H2.
+ auto.
+Qed.
+Hint Resolve wffs_sregion_cons.
+
